\newcommand{\sheet}{2}
\input{Header.tex}

\begin{document}

\maketitle{}

\begin{exercise}{4}
    For $i \leq -1$ we define $h_i = 0$.

    Since the chain is exact, the map $d_1$ must be surjective. Therefore we can
    define $h_0$ as the lift of $\id \colon C_0 \to C_0$ along surjection $d_1
    \colon C_1 \to C_0$. (Though there was no need to treat this case separately)

    Let now $i \geq 1$ and suppose $h_j$ for $j < i$ exist with property as in the exercise.
    Observe that $\id_{C_i} - h_{i-1} \circ d_i \colon C_i \to C_i$ factors
    through $\ker(d_i)$, since
    \begin{equation*}
        \begin{split}
            d_i \circ (\id_{C_i} - h_{i-1} \circ d_i) &= d_i - d_i \circ h_{i-1}
            \circ d_i \\
            &= d_i - (id_{C_{i-1}} - h_{i-2} \circ d_{i-1}) \circ d_i \\
            &= d_i - d_i \\
            &= 0.
        \end{split}
    \end{equation*}
    Using exactness ($\im(d_{i+1}) = \ker(d_i)$), we can lift $C_i \to
    \im(d_{i+1})$ along the surjection $C_{i+1} \to \im(d_{i+1})$ to obtain $h_i
    \colon C_i \to C_{i+1}$ for which $d_{i+1} \circ h_i = \id_{C_i} - h_{i-1}
    \circ d_i$.

\end{exercise}

\end{document}
